code/k256/Hacl.K256.Scalar.fsti
@@ -54,14 +54,12 @@ val create_qelem: unit -> StackInline qelem
     qas_nat h1 f == 0)
 
 
-inline_for_extraction noextract
 val is_qelem_zero_vartime (f:qelem) : Stack bool
   (requires fun h -> live h f)
   (ensures  fun h0 m h1 -> modifies0 h0 h1 /\
     m == (qas_nat h0 f = 0))
 
 
-inline_for_extraction noextract
 val is_qelem_eq_vartime (f1 f2:qelem) : Stack bool
   (requires fun h ->
     live h f1 /\ live h f2 /\ qe_lt_q h f1 /\ qe_lt_q h f2)
@@ -89,15 +87,8 @@ val load_qelem_modq: f:qelem -> b:lbuffer uint8 32ul -> Stack unit
   (requires fun h ->
     live h f /\ live h b /\ disjoint f b)
   (ensures  fun h0 _ h1 -> modifies (loc f) h0 h1 /\
-    qas_nat h1 f == BSeq.nat_from_bytes_be (as_seq h0 b) % S.q)
-
-
-val qelem_from_felem: out:qelem -> f:F.felem -> Stack unit
-  (requires fun h ->
-    live h out /\ live h f /\ eq_or_disjoint out f)
-  (ensures  fun h0 _ h1 -> modifies (loc out) h0 h1 /\
-    qas_nat h1 out == F.as_nat h0 f % S.q /\
-    qe_lt_q h1 out)
+    qas_nat h1 f == BSeq.nat_from_bytes_be (as_seq h0 b) % S.q /\
+    qe_lt_q h1 f)
 
 
 val store_qelem: b:lbuffer uint8 32ul -> f:qelem -> Stack unit
@@ -106,15 +97,6 @@ val store_qelem: b:lbuffer uint8 32ul -> f:qelem -> Stack unit
     qe_lt_q h f)
   (ensures  fun h0 _ h1 -> modifies (loc b) h0 h1 /\
     as_seq h1 b == BSeq.nat_to_bytes_be 32 (qas_nat h0 f))
-
-
-// not used
-inline_for_extraction noextract
-val copy_qelem (f1 f2: qelem) : Stack unit
-  (requires fun h ->
-    live h f1 /\ live h f2 /\ disjoint f1 f2)
-  (ensures  fun h0 _ h1 -> modifies (loc f1) h0 h1 /\
-    as_seq h1 f1 == as_seq h0 f2)
 
 
 val qadd (out f1 f2: qelem) : Stack unit
